LL1/CompletenessProof.v
@@ -1,381 +1,324 @@
 Require Import List Omega String.
 Require Import Derivation Grammar Lemmas ParseTable
         ParseTree LL1.Parser Lib.Tactics
-        LL1.CorrectnessProof.
+        LL1.CorrectnessProof LL1.MonotonicityLemmas.
 
-Lemma forest_fuel_tree_S_fuel :
-  forall g tbl gamma input fuel suffix subtrees ntName,
+Conjecture in_grammar_lookup :
+  forall tbl g x gamma,
     isParseTableFor tbl g
-    -> In (NT ntName, gamma) g
-    -> parseForest tbl gamma input fuel =
-       (Some subtrees, suffix)
-    -> parse tbl (NT ntName) input (S fuel) =
-       (Some (Node ntName subtrees), suffix).
+    -> In (x, gamma) g.(productions)
+    -> exists lk,
+        parseTableLookup x lk tbl = Some gamma.
+
+Lemma symbol_eq_dec :
+  forall (s s2 : symbol),
+    {s = s2} + {~s = s2}.
+Proof. repeat decide equality. Qed.
+
+Conjecture lookup_deterministic :
+  forall tbl g x lk lk',
+    isParseTableFor tbl g
+    ->
+    (parseTableLookup x lk tbl = parseTableLookup x lk' tbl
+     <-> lk = lk').
+
+Ltac sim := simpl in *.
+
+Definition beqSymTy s s2 :=
+  match (s, s2) with
+  | (T _, T _) => true
+  | (NT _, NT _) => true
+  | _ => false
+  end.
+
+Lemma lookup_det :
+  forall tbl g lk x x',
+    isParseTableFor tbl g
+    -> parseTableLookup x lk tbl =
+       parseTableLookup x' lk tbl
+    -> x = x'.
 Proof.
   intros.
-  destruct fuel as [| fuel].
-  - inv H1.
-  - destruct gamma as [| sym gamma'].
-    + (* gamma is nil *)
-      simpl in H1. (* now we know that parseForest
-                      produces an empty list of subtrees *)
-      inv H1.
-      destruct suffix as [| token suffix'].
-      * simpl.
-        (* The problem is that there's no lookahead token,
-           which isn't a problem for parseForest, but IS a
-           problem for parse *)
-Abort.
-      
-Conjecture forest_fuel_tree_S_fuel :
-  forall tbl gamma input fuel suffix subtrees ntName,
-    parseForest tbl gamma input fuel =
-    (Some subtrees, suffix)
-    -> parse tbl (NT ntName) input (S fuel) =
-       (Some (Node ntName subtrees), suffix).
+  unfold parseTableLookup in H0.
+Abort. (* Not true, I don't think
+          X -> aY
+          X -> bZ
+          Y -> c
+          Z -> c *)
 
-Lemma parse_fuel_monotonic :
-  forall tr tbl sym input suffix fuel fuel2,
-    parse tbl sym input fuel = (Some tr, suffix)
-    -> fuel < fuel2
-    -> parse tbl sym input fuel2 = (Some tr, suffix).
+Lemma lookup_diff :
+  forall tbl g lk x x',
+    isParseTableFor tbl g
+    -> x <> x'
+    -> parseTableLookup x lk tbl <>
+       parseTableLookup x' lk tbl.
 Proof.
-  induction tr as [ s
+  unfold not; intros.
+  apply H0; clear H0. 
+Abort.                      
+
+Conjecture det :
+  forall tbl g gamma gamma' input fuel,
+    isParseTableFor tbl g
+    -> parseForest tbl gamma input fuel =
+       parseForest tbl gamma' input fuel
+    -> gamma = gamma'.
+
+Conjecture step :
+  forall tbl g gamma input fuel f suffix x,
+    isParseTableFor tbl g
+    -> In (x, gamma) g.(productions)
+    -> parseForest tbl gamma input fuel = (Some f, suffix)
+    <-> parse tbl (NT x) input (S fuel) =
+        (Some (Node x f), suffix).
+
+Lemma lookup_ok :
+  forall tbl g x gamma input fuel f suffix,
+    isParseTableFor tbl g
+    -> In (x, gamma) g.(productions)
+    -> parseForest tbl gamma input fuel = (Some f, suffix)
+    -> parseTableLookup x (peek input) tbl = Some gamma.
+Proof.
+  intros.
+  remember H1 as H1'; clear HeqH1'.
+  apply step with (g := g) (x := x) in H1.
+  - simpl in H1.
+    destruct (parseTableLookup x (peek input) tbl)
+      as [gamma' |] eqn:Hlkp.
+    + destruct (parseForest tbl gamma' input fuel)
+               as (subresult, input') eqn:Hpf.
+      destruct subresult as [f' |].
+      * inv H1.
+        rewrite <- Hpf in H1'.
+        eapply det in H1'. (* NEED TO PROVE THIS! *)
+        { subst. trivial. }
+        { eauto. }
+      * inv H1.
+    + inv H1.
+  - trivial.
+  - trivial.
+Qed.
+          
+Lemma unfold_parse :
+  forall tbl x input fuel,
+    parse tbl (NT x) input (S fuel) =
+    match parseTableLookup x (peek input) tbl with
+    | None => (None, input)
+    | Some gamma =>
+      match parseForest tbl gamma input fuel with
+      | (None, _) => (None, input)
+      | (Some sts, input') =>
+        (Some (Node x sts), input')
+      end
+    end.
+Proof.
+  trivial.
+Qed.
+
+
+Conjecture lookup_parseForest :
+  forall tbl g x gamma input fuel f suffix,
+    isParseTableFor tbl g
+    -> In (x, gamma) g.(productions)
+    -> parseForest tbl gamma input fuel =
+       (Some f, suffix)
+    -> parseTableLookup x (peek input) tbl = Some gamma.
+
+Lemma at_most_one_sym_succeeds :
+  forall tbl g,
+    isParseTableFor tbl g
+    -> forall tr x input fuel suffix,
+      parse tbl (NT x) input fuel = (Some tr, suffix)
+      -> forall x' tr' suffix',
+        x <> x'
+        -> ~parse tbl (NT x') input fuel =
+           (Some tr', suffix').
+Proof.
+  intros tbl g Htbl.
+    induction tr as [ s
                   | s f IHparseForest
                   |
                   | tr IHparse f IHparseForest ]
       using tree_mutual_ind with
-      (P := fun tr =>
-              forall tbl sym input suffix fuel fuel2,
-                parse tbl sym input fuel = (Some tr, suffix)
-                -> fuel < fuel2
-                -> parse tbl sym input fuel2 =
-                   (Some tr, suffix))
-      (P0 := fun subtrees =>
-               forall tbl gamma input suffix fuel fuel2,
-                 parseForest tbl gamma input fuel =
-                 (Some subtrees, suffix)
-                 -> fuel < fuel2
-                 -> parseForest tbl gamma input fuel2 =
-                    (Some subtrees, suffix)).
+        (P := fun tr =>
+                forall x input fuel suffix,
+                  parse tbl (NT x) input fuel =
+                  (Some tr, suffix)
+                -> forall x' tr' suffix',
+                  x <> x'
+                  -> ~parse tbl (NT x') input fuel =
+                     (Some tr', suffix'))
+        
+        (P0 := fun subtrees =>
+                 forall gamma input fuel suffix,
+                   parseForest tbl gamma input fuel =
+                   (Some subtrees, suffix)
+                   -> forall gamma' subtrees' suffix',
+                     gamma <> gamma'
+                     -> ~parseForest tbl gamma' input fuel =
+                        (Some subtrees', suffix)).
+
+
+  - unfold not; intros.
+    apply H0.
+    destruct fuel; sim.
+    + inv H.
+    + destruct (parseTableLookup x (peek input) tbl)
+        as [gamma |] eqn:Hlkp;
+        destruct (parseTableLookup x' (peek input) tbl)
+        as [gamma' |] eqn:Hlkp'.
+      * destruct (parseForest tbl gamma input fuel)
+          as (o, input') eqn:Hpf.
+        destruct (parseForest tbl gamma' input fuel)
+          as (o', input'').
+        destruct o; destruct o'.
+        { inv H. }
+        { inv H. }
+        { inv H. }
+        { inv H. }
+      * inv H1.
+      * inv H.
+      * inv H.
+
+  - unfold not; intros.
+    destruct fuel; sim.
+    + inv H.
+    + destruct (parseTableLookup x (peek input) tbl)
+        as [gamma |] eqn:Hlkp;
+      destruct (parseTableLookup x' (peek input) tbl)
+        as [gamma' |] eqn:Hlkp'.
+      * destruct (parseForest tbl gamma input fuel)
+          as (o, input') eqn:Hpf.
+        destruct (parseForest tbl gamma' input fuel)
+          as (o', input'') eqn:Hpf'.
+        destruct o; destruct o'.
+        { inv H.
+          inv H1.
+          eapply IHparseForest.
+          { eapply Hpf. }
+          { eauto. }
+          { unfold not; intros.
+            apply H0.
+            rewrite <- H in Hpf'.
+            rewrite Hpf in Hpf'.
+            inv Hpf'.
+            rewrite <- Hlkp in Hlkp'.
+Abort. (* seems promising, though *)
+
+
+Lemma derivesTree_lookup :
+  forall g x prefix f,
+    (@derivesTree g) (NT x) prefix (Node x f)
+    -> forall tbl x suffix gamma,
+    isParseTableFor tbl g
+      -> parseTableLookup x (peek (prefix ++ suffix)) tbl =
+         Some gamma.
+Proof.
+  intros g x prefix f H.
+  inv H.
+  intros.
+  destruct prefix.
+  - simpl.
+Abort.
+
+Lemma derives_exists :
+  forall g x input trees,
+    (@derivesTree g) (NT x) input (Node x trees)
+    -> exists gamma,
+      In (x, gamma) (productions g)
+      /\ (@derivesForest g) gamma input trees.
+Proof.
+  intros.
+  inv H.
+  exists gamma; split; trivial.
+Qed.
+
+Lemma der_lookup :
+  forall tbl g,
+    isParseTableFor tbl g
+    -> forall trees x input gamma,
+      (@derivesTree g) (NT x) input (Node x trees)
+      -> (@derivesForest g) gamma input trees
+      -> parseTableLookup x (peek input) tbl = Some gamma.
+Proof.
+  intros tbl g Htbl trees.
+  unfold isParseTableFor in Htbl.
+  destruct Htbl as [Hcom Hmin].
+  destruct Hcom as [Hcomfi Hcomfo].
+  unfold ptCompleteFirst in Hcomfi.
+  unfold ptCompleteFollow in Hcomfo.
+  induction trees as [| tr trs]; intros.
+  - inv H.
+    inv H0.
+    inv H5.
+    simpl in *.
+
+Lemma dd :
+  forall trees g gamma prefix suffix x tbl,
+    (@derivesForest g) gamma prefix trees
+    -> (@derivesTree g) (NT x) prefix (Node x trees)
+    -> isParseTableFor tbl g
+    -> parseTableLookup x (peek (app prefix suffix)) tbl =
+       Some gamma.
+Proof.
+  induction trees as [| st sts]; intros.
+  - inv H.
+    inv H0.
+    inv H5.
+    simpl.
+    unfold isParseTableFor in H1.
+    destruct H1 as [Hcom Hmin].
+    unfold parseTableComplete in Hcom.
+    destruct Hcom as [Hcomfi Hcomfo].
+    unfold ptCompleteFollow in Hcomfo.
+    
+    apply Hcomfo with (y := EOF) in H3.
+    + destruct H3 as [tMap [H3 H4]].
+      unfold parseTableLookup.
+      rewrite H3.
+      trivial.
+Admitted.
+
+Lemma in_grammar_lookup_tbl :
+  forall tbl g,
+    isParseTableFor tbl g
+    -> forall gamma prefix suffix x fuel f,
+      In (x, gamma) (productions g)
+      -> parseForest tbl gamma (app prefix suffix) fuel =
+         (Some f, suffix)
+      -> parseTableLookup x (peek (app prefix suffix)) tbl =
+         Some gamma.
+Proof.
+  intros tbl g Htbl gamma.
+  intros.
+  assert (H1 : exists (prefix' : list string),
+               (app prefix' suffix) = (app prefix suffix)
+               /\ (@derivesForest g) gamma prefix' f).
+  { admit. }
+  destruct H1 as [prefix' [H1 H2]].
+  assert (prefix' = prefix).
+  { admit. }
+  subst.
+  assert ((@derivesTree g) (NT x) prefix (Node x f)).
+  { eapply derivesNT; eauto. }
+  apply derives_exists in H3.
+
+    
+  induction gamma as [| sym syms]; intros.
+Abort.
   
-  - intros tbl sym input suffix fuel fuel2 Hparse Hfuel.
-    destruct fuel.
-    + inv Hparse.
-    + destruct fuel2.
-      * inv Hfuel.
-      * destruct sym as [y | x].
-        { destruct input as [| token tokens].
-          { inv Hparse. }
-          { simpl; simpl in Hparse.
-            destruct (Utils.beqSym (T y) (T token)).
-            { inv Hparse. reflexivity. }
-            { inv Hparse. }}}
-        { apply nt_derives_Node in Hparse. inv Hparse. }
+        
+Conjecture in_grammar_lookup_tbl :
+  forall tbl g,
+    isParseTableFor tbl g
+    -> forall x gamma prefix suffix fuel f,
+      In (x, gamma) (productions g)
+      -> parseForest tbl gamma (app prefix suffix) fuel =
+         (Some f, suffix)
+      -> parseTableLookup x (peek (app prefix suffix)) tbl =
+         Some gamma.
 
-  - intros tbl sym input suffix fuel fuel2 Hparse Hfuel.
-    destruct fuel.
-    + inv Hparse.
-    + destruct fuel2.
-      * inv Hfuel.
-      * destruct sym as [y | x].
-        { apply t_derives_Leaf in Hparse. inv Hparse. }
-        { destruct input as [| token tokens].
-          { inv Hparse. }
-          { simpl; simpl in Hparse.
-            destruct (parseTableLookup (NT x) (T token) tbl)
-              as [gamma |].
-            { destruct (parseForest tbl
-                                    gamma
-                                    (token :: tokens)
-                                    fuel)
-                as (subresult, input') eqn:HpfFuel.
-              destruct subresult as [subtrees |].
-              { destruct (parseForest tbl
-                                      gamma
-                                      (token :: tokens)
-                                      fuel2)
-                  as (subresult, input'') eqn:HpfFuel2.
-                destruct subresult as [subtrees' |].
-                { inv Hparse.
-                  apply IHparseForest with (fuel2 := fuel2)
-                    in HpfFuel.
-                  { rewrite HpfFuel in HpfFuel2.
-                    inv HpfFuel2.
-                    reflexivity. }
-                  { omega. }}
-                { inv Hparse.
-                  apply IHparseForest with (fuel2 := fuel2)
-                    in HpfFuel.
-                  { rewrite HpfFuel in HpfFuel2.
-                    inv HpfFuel2. }
-                  { omega. }}}
-              { inv Hparse. }}
-            { inv Hparse. }}}
-
-  - intros tbl gamma input suffix fuel fuel2 Hparse Hfuel.
-    destruct fuel.
-    + inv Hparse.
-    + destruct fuel2.
-      * inv Hfuel.
-      * destruct gamma as [| sym syms].
-        { simpl. inv Hparse. reflexivity. }
-        (* Maybe prove in a separate lemma that 
-           a non-empty gamma never derives Fnil *)
-        { simpl in Hparse.
-          destruct (parse tbl sym input fuel)
-            as (subresult, input').
-          destruct subresult as [lSib |].
-          { destruct (parseForest tbl syms input' fuel)
-              as (subresult, input'').
-            destruct subresult as [rSibs |].
-            { inv Hparse. }
-            { inv Hparse. }}
-          { inv Hparse. }}
-
-  - intros tbl gamma input suffix fuel fuel2 Hparse Hfuel.
-    destruct fuel.
-    + inv Hparse.
-    + destruct fuel2.
-      * inv Hfuel.
-      * destruct gamma as [| sym syms].
-        { inv Hparse. }
-        { simpl; simpl in Hparse.
-          destruct (parse tbl sym input fuel)
-            as (subresult, input') eqn:HparseFuel.
-          { destruct subresult as [lSib |].
-            { destruct (parseForest tbl syms input' fuel)
-                as (subresult, input'') eqn:HparseForestFuel.
-              destruct subresult as [rSibs |].
-              { destruct (parse tbl sym input fuel2)
-                  as (subresult, input2') eqn:HparseFuel2.
-                { destruct subresult as [lSib2 |].
-                  { destruct (parseForest tbl syms input2' fuel2) as (subresult, input2'') eqn:HparseForestFuel2.
-                    destruct subresult as [rSibs2 |].
-                    { inv Hparse.
-                      apply IHparse with (fuel2 := fuel2)
-                        in HparseFuel.
-                      { rewrite HparseFuel in HparseFuel2.
-                        inv HparseFuel2.
-                        apply IHparseForest
-                          with (fuel2 := fuel2)
-                          in HparseForestFuel.
-                        { rewrite HparseForestFuel in HparseForestFuel2.
-                          inv HparseForestFuel2.
-                          reflexivity. }
-                        { omega. }}
-                      { omega. }}
-                    { inv Hparse.
-                      apply IHparse
-                        with (fuel2 := fuel2)
-                        in HparseFuel.
-                      { rewrite HparseFuel in HparseFuel2.
-                        inv HparseFuel2.
-                        apply IHparseForest
-                          with (fuel2 := fuel2)
-                        in HparseForestFuel.
-                        { rewrite HparseForestFuel
-                          in HparseForestFuel2.
-                          inv HparseForestFuel2. }
-                        { omega. }}
-                      { omega. }}}
-                  { inv Hparse.
-                    apply IHparse
-                      with (fuel2 := fuel2)
-                      in HparseFuel.
-                    { rewrite HparseFuel in HparseFuel2.
-                      inv HparseFuel2. }
-                    { omega. }}}}
-              { inv Hparse. }}
-            { inv Hparse. }}}
-Qed.
-
-Lemma parseForest_fuel_monotonic :
-  forall sts tbl gamma input suffix fuel fuel2,
-    parseForest tbl gamma input fuel = (Some sts, suffix)
-    -> fuel < fuel2
-    -> parseForest tbl gamma input fuel2 = (Some sts, suffix).
-Proof.
-  induction sts as [ s
-                   | s f IHparseForest
-                   |
-                   | tr IHparse f IHparseForest ]
-      using forest_mutual_ind with
-      (P := fun tr =>
-              forall tbl sym input suffix fuel fuel2,
-                parse tbl sym input fuel = (Some tr, suffix)
-                -> fuel < fuel2
-                -> parse tbl sym input fuel2 =
-                   (Some tr, suffix))
-      (P0 := fun subtrees =>
-               forall tbl gamma input suffix fuel fuel2,
-                 parseForest tbl gamma input fuel =
-                 (Some subtrees, suffix)
-                 -> fuel < fuel2
-                 -> parseForest tbl gamma input fuel2 =
-                    (Some subtrees, suffix)).
-  
-  - intros tbl sym input suffix fuel fuel2 Hparse Hfuel.
-    destruct fuel.
-    + inv Hparse.
-    + destruct fuel2.
-      * inv Hfuel.
-      * destruct sym as [y | x].
-        { destruct input as [| token tokens].
-          { inv Hparse. }
-          { simpl; simpl in Hparse.
-            destruct (Utils.beqSym (T y) (T token)).
-            { inv Hparse. reflexivity. }
-            { inv Hparse. }}}
-        { apply nt_derives_Node in Hparse. inv Hparse. }
-
-  - intros tbl sym input suffix fuel fuel2 Hparse Hfuel.
-    destruct fuel.
-    + inv Hparse.
-    + destruct fuel2.
-      * inv Hfuel.
-      * destruct sym as [y | x].
-        { apply t_derives_Leaf in Hparse. inv Hparse. }
-        { destruct input as [| token tokens].
-          { inv Hparse. }
-          { simpl; simpl in Hparse.
-            destruct (parseTableLookup (NT x) (T token) tbl)
-              as [gamma |].
-            { destruct (parseForest tbl
-                                    gamma
-                                    (token :: tokens)
-                                    fuel)
-                as (subresult, input') eqn:HpfFuel.
-              destruct subresult as [subtrees |].
-              { destruct (parseForest tbl
-                                      gamma
-                                      (token :: tokens)
-                                      fuel2)
-                  as (subresult, input'') eqn:HpfFuel2.
-                destruct subresult as [subtrees' |].
-                { inv Hparse.
-                  apply IHparseForest with (fuel2 := fuel2)
-                    in HpfFuel.
-                  { rewrite HpfFuel in HpfFuel2.
-                    inv HpfFuel2.
-                    reflexivity. }
-                  { omega. }}
-                { inv Hparse.
-                  apply IHparseForest with (fuel2 := fuel2)
-                    in HpfFuel.
-                  { rewrite HpfFuel in HpfFuel2.
-                    inv HpfFuel2. }
-                  { omega. }}}
-              { inv Hparse. }}
-            { inv Hparse. }}}
-
-  - intros tbl gamma input suffix fuel fuel2 Hparse Hfuel.
-    destruct fuel.
-    + inv Hparse.
-    + destruct fuel2.
-      * inv Hfuel.
-      * destruct gamma as [| sym syms].
-        { simpl. inv Hparse. reflexivity. }
-        (* Maybe prove in a separate lemma that 
-           a non-empty gamma never derives Fnil *)
-        { simpl in Hparse.
-          destruct (parse tbl sym input fuel)
-            as (subresult, input').
-          destruct subresult as [lSib |].
-          { destruct (parseForest tbl syms input' fuel)
-              as (subresult, input'').
-            destruct subresult as [rSibs |].
-            { inv Hparse. }
-            { inv Hparse. }}
-          { inv Hparse. }}
-
-  - intros tbl gamma input suffix fuel fuel2 Hparse Hfuel.
-    destruct fuel.
-    + inv Hparse.
-    + destruct fuel2.
-      * inv Hfuel.
-      * destruct gamma as [| sym syms].
-        { inv Hparse. }
-        { simpl; simpl in Hparse.
-          destruct (parse tbl sym input fuel)
-            as (subresult, input') eqn:HparseFuel.
-          { destruct subresult as [lSib |].
-            { destruct (parseForest tbl syms input' fuel)
-                as (subresult, input'') eqn:HparseForestFuel.
-              destruct subresult as [rSibs |].
-              { destruct (parse tbl sym input fuel2)
-                  as (subresult, input2') eqn:HparseFuel2.
-                { destruct subresult as [lSib2 |].
-                  { destruct (parseForest tbl syms input2' fuel2) as (subresult, input2'') eqn:HparseForestFuel2.
-                    destruct subresult as [rSibs2 |].
-                    { inv Hparse.
-                      apply IHparse with (fuel2 := fuel2)
-                        in HparseFuel.
-                      { rewrite HparseFuel in HparseFuel2.
-                        inv HparseFuel2.
-                        apply IHparseForest
-                          with (fuel2 := fuel2)
-                          in HparseForestFuel.
-                        { rewrite HparseForestFuel in HparseForestFuel2.
-                          inv HparseForestFuel2.
-                          reflexivity. }
-                        { omega. }}
-                      { omega. }}
-                    { inv Hparse.
-                      apply IHparse
-                        with (fuel2 := fuel2)
-                        in HparseFuel.
-                      { rewrite HparseFuel in HparseFuel2.
-                        inv HparseFuel2.
-                        apply IHparseForest
-                          with (fuel2 := fuel2)
-                        in HparseForestFuel.
-                        { rewrite HparseForestFuel
-                          in HparseForestFuel2.
-                          inv HparseForestFuel2. }
-                        { omega. }}
-                      { omega. }}}
-                  { inv Hparse.
-                    apply IHparse
-                      with (fuel2 := fuel2)
-                      in HparseFuel.
-                    { rewrite HparseFuel in HparseFuel2.
-                      inv HparseFuel2. }
-                    { omega. }}}}
-              { inv Hparse. }}
-            { inv Hparse. }}}
-Qed. (* Hmm...same proof as the one for parse! *)
-
-Lemma parse_fuel_max :
-  forall fuel tbl sym input fuel2 tr suffix,
-    parse tbl sym input fuel = (Some tr, suffix) ->
-    parse tbl sym input (max fuel fuel2) = (Some tr, suffix).
-Proof.
-  intros. 
-  pose proof (Max.max_spec fuel fuel2) as H_max_spec.
-  destruct H_max_spec.
-  - destruct H0. rewrite H1.
-    eapply parse_fuel_monotonic.
-    + eassumption.
-    + assumption.
-  - destruct H0. rewrite H1. assumption.
-Qed.
-
-Lemma parseForest_fuel_max :
-  forall tbl gamma input fuel fuel2 sts suffix,
-    parseForest tbl gamma input fuel = (Some sts, suffix)
-    -> parseForest tbl gamma input (max fuel fuel2) =
-       (Some sts, suffix).
-Proof.
-  intros. pose proof (Max.max_spec fuel fuel2) as H_max_spec.
-  destruct H_max_spec.
-  - destruct H0. rewrite H1.
-    eapply parseForest_fuel_monotonic.
-    + eassumption.
-    + assumption.
-  - destruct H0. rewrite H1. assumption.
-Qed.
-
+(*
 Theorem parse_complete :
   forall (g   : grammar)
          (tbl : parse_table),
@@ -386,8 +329,14 @@ Theorem parse_complete :
            (prefix suffix : list string),
       input = (prefix ++ suffix)%list ->
       (@derivesTree g) sym prefix tr ->
-      exists (fuel : nat),
-        parse tbl sym input fuel = (Some tr, suffix).
+      match tr with
+      | (Leaf y) => exists fuel,
+                    parse tbl sym input fuel = (Some tr, suffix)
+      | (Node x f) => exists fuel fuel2 gamma,
+                      parseTableLookup x (peek input) tbl = Some gamma
+                      /\ parseForest tbl gamma input fuel = (Some f, suffix)
+                      /\ parse tbl sym input fuel2 = (Some tr, suffix)
+      end.
 Proof.
   intros g tbl Htbl tr.
   induction tr as [ s
@@ -397,52 +346,130 @@ Proof.
       using tree_mutual_ind with
       (P := fun tr =>
               forall input sym prefix suffix,
-                input = (prefix ++ suffix)%list ->
-                (@derivesTree g) sym prefix tr ->
-                exists (fuel : nat),
-                  parse tbl sym input fuel = (Some tr, suffix))
+              input = (prefix ++ suffix)%list ->
+              (@derivesTree g) sym prefix tr ->
+              match tr with
+              | (Leaf y) => exists fuel,
+                            parse tbl sym input fuel = (Some tr, suffix)
+              | (Node x f) => exists fuel fuel2 gamma,
+                              parseTableLookup x (peek input) tbl = Some gamma
+                              /\ parseForest tbl gamma input fuel = (Some f, suffix)
+                              /\ parse tbl sym input fuel2 = (Some tr, suffix)
+              end)
       (P0 := fun subtrees =>
                forall input gamma prefix suffix,
-                 input = (prefix ++ suffix)%list ->
-                 (@derivesForest g) gamma prefix subtrees ->
-                 exists fuel,
-                   parseForest tbl gamma input fuel = (Some subtrees, suffix)).
-  
+                     input = (prefix ++ suffix)%list ->
+                     (@derivesForest g) gamma prefix subtrees ->
+                     exists x fuel, parseTableLookup x (peek input) tbl= Some gamma
+                                    /\ parseForest tbl gamma input fuel = (Some subtrees, suffix)).
+
+  - intros.
+    inv H0.
+    exists 1.
+    simpl.
+    assert (Utils.beqString s s = true) by admit.
+    rewrite H.
+    trivial.
+
+  - intros.
+    inv H0.
+    eapply IHparseForest with (prefix := prefix) (suffix := suffix) (input := app prefix suffix) in H6.
+    + destruct H6 as [x [fuel [ Hl Hpf]]].
+      exists fuel. exists (S fuel). exists gamma.
+      split.
+      * trivial.
+*)
+
+Theorem parse_complete :
+  forall (g   : grammar)
+         (tbl : parse_table),
+    isParseTableFor tbl g ->
+    forall (tr     : tree)
+           (input  : list string)
+           (sym    : symbol)
+           (prefix suffix : list string),
+      input = (prefix ++ suffix)%list ->
+      derivesMaximalTree g sym prefix suffix tr
+      -> exists (fuel : nat),
+          parse tbl sym input fuel = (Some tr, suffix).
+Proof.
+  intros g tbl Htbl tr.
+  induction tr as [ s
+                  | s f IHparseForest
+                  |
+                  | tr IHparse f IHparseForest ]
+                    using tree_mutual_ind with
+      
+      (P := fun tr =>
+              forall input sym prefix suffix,
+                input = (prefix ++ suffix)%list ->
+                derivesMaximalTree g sym prefix suffix tr
+                -> exists (fuel : nat),
+                    parse tbl sym input fuel =
+                    (Some tr, suffix))
+
+      (P0 := fun subtrees =>
+               forall input gamma prefix suffix,
+                 input = (prefix ++ suffix)%list
+                 -> (@derivesForest g) gamma prefix subtrees
+                 -> exists fuel,
+                     parseForest tbl gamma input fuel =
+                     (Some subtrees, suffix)).
+
   - intros input sym prefix suffix Hinput HderivesTree.
     inv HderivesTree.
+    inv H.
     exists 1. simpl.
-    destruct (Utils.beqSym (T s) (T s)) eqn:Hbeq.
+    destruct (Utils.beqString s s) eqn:Hbeq.
     + reflexivity.
-    + unfold Utils.beqSym in Hbeq.
-      destruct (SymbolMapFacts.eq_dec) in Hbeq.
+    + unfold Utils.beqString in Hbeq.
+      destruct (StringMapFacts.eq_dec) in Hbeq.
       * inv Hbeq.
       * exfalso. apply n. reflexivity.
-        
+
+  (* hard case *)
   - intros input sym prefix suffix Hinput HderivesTree.
     inv HderivesTree.
+    inv H.
     apply IHparseForest with (prefix := prefix)
                              (suffix := suffix)
                              (input := app prefix suffix)
-      in H4; clear IHparseForest.
+      in H6; clear IHparseForest; eauto.
+    destruct H6 as [fuel].
+    
     + destruct H4 as [fuel].
       exists (S fuel).
-      eapply forest_fuel_tree_S_fuel. eassumption.
-    + reflexivity.
-      
-  - intros input gamma prefix suffix Hinput HderivesForest.
+      simpl.
+      destruct (parseTableLookup s
+                                 (peek (prefix ++ suffix)) tbl)
+        as [gamma' |] eqn:Hlkp.
+      * destruct (parseForest tbl gamma' (prefix ++ suffix)
+                              fuel)
+          as (o, suffix') eqn:Hpf.
+        destruct o as [f' |].
+        -- unfold parseTableLookup in Hlkp.
+           
+      eapply in_grammar_lookup_tbl in Htbl; eauto.
+      rewrite Htbl.
+      rewrite H.
+      trivial.
+
+  - intros x input gamma prefix suffix Hinput HderivesForest.
     inv HderivesForest.
-    exists 1. simpl. reflexivity.
-    
-  - intros input gamma prefix suffix Hinput HderivesForest.
+    exists 1. simpl. trivial.
+      
+  - intros x input gamma prefix suffix Hinput HderivesForest.
     inv HderivesForest.
     apply IHparse with
         (input := ((prefix0 ++ suffix0)%list ++ suffix)%list)
         (suffix := (suffix0 ++ suffix)%list) in H3;
       clear IHparse.
     + destruct H3 as [hdFuel].
+      
       apply IHparseForest with
       (input := (suffix0 ++ suffix)%list)
-          (suffix := suffix) in H4; clear IHparseForest.
+      (suffix := suffix)
+       in H4; clear IHparseForest.
       * destruct H4 as [tlFuel].
         apply parse_fuel_max with (fuel2 := tlFuel) in H.
         apply parseForest_fuel_max
@@ -463,9 +490,14 @@ Proof.
             as (subresult, input'') eqn:H_tl.
           destruct subresult as [rSibs |].
           { inv H. rewrite H0 in H_tl.
-            inv H_tl. reflexivity. }
-          { inv H. rewrite H0 in H_tl. inv H_tl. }}
+            inv H_tl.
+            split; try trivial. }
+          { inv H. congruence. }}
         { inv H. }
-      * reflexivity.
+      * trivial.
+      * trivial.
     + rewrite <- app_assoc. reflexivity.
 Qed.
+
+(* - Doing induction on the right thing?
+   - Look at example of inductive proof using fuel *)
