LL1/InGrammarLookupTbl.v
@@ -1,0 +1,689 @@
+Require Import LL1.Parser ParseTable Derivation Grammar ParseTree Lib.Tactics LL1.CorrectnessProof.
+Require Import List String.
+Import ListNotations.
+
+Inductive nullableProd {g : grammar} :
+  nonterminal -> list symbol -> Prop :=
+| n_prod :
+    forall x ys,
+      In (x, ys) g.(productions)
+      -> nullableGamma ys
+      -> nullableProd x ys
+with nullableGamma {g : grammar} :
+       list symbol -> Prop :=
+     | n_nil :
+         nullableGamma nil
+     | n_cons :
+         forall x tl,
+           nullableSym x
+           -> nullableGamma tl
+           -> nullableGamma (NT x :: tl)
+with nullableSym {g : grammar} :
+       nonterminal -> Prop :=
+     | n_sym :
+         forall x ys,
+           nullableProd x ys
+           -> nullableSym x.
+
+Inductive firstProd {g : grammar} :
+    lookahead -> nonterminal -> list symbol -> Prop :=
+| first_prod : forall la x gamma,
+    In (x, gamma) g.(productions)
+    -> firstGamma la gamma
+    -> firstProd la x gamma
+with firstGamma {g : grammar} :
+       lookahead -> list symbol -> Prop :=
+     | fgamma_hd : forall la hd tl,
+         firstSym la hd ->
+         firstGamma la (hd :: tl)
+     | fgamma_tl : forall la x tl,
+         (@nullableSym g) x ->
+         firstGamma la tl ->
+         firstGamma la (NT x :: tl)
+with firstSym {g : grammar} :
+       lookahead -> symbol -> Prop :=
+| first_t : forall s,
+    firstSym (LA s) (T s)
+| first_nt : forall la x gamma,
+    firstProd la x gamma ->
+    firstSym la (NT x).
+
+Inductive followProd {g : grammar} :
+  lookahead -> nonterminal -> list symbol -> Prop :=
+| follow_prod :
+    forall la x gamma,
+      In (x, gamma) g.(productions)
+      -> followSym la x
+      -> followProd la x gamma
+with followSym {g : grammar} :
+       lookahead -> nonterminal -> Prop :=
+     | f_start :
+         followSym EOF g.(start)
+     | f_right :
+         forall x1 x2 prefix suffix la,
+           In (x1, prefix ++ NT x2 :: suffix) g.(productions)
+           -> (@firstGamma g) la suffix
+           -> followSym la x2
+     | f_left :
+         forall x1 x2 prefix suffix la,
+           In (x1, prefix ++ NT x2 :: suffix) g.(productions)
+           -> (@nullableGamma g) suffix
+           -> followSym la x1
+           -> followSym la x2.
+
+Definition isLookaheadFor {g} la x gamma :=
+  (@firstProd g) la x gamma
+  \/ (@nullableProd g) x gamma /\ (@followProd g) la x gamma.
+
+Definition ptMinimal tbl g :=
+  forall x la gamma laMap,
+    StringMap.find x tbl = Some laMap
+    -> LookaheadMap.find la laMap = Some gamma
+    -> (@isLookaheadFor g) la x gamma.
+
+Definition ptComplete tbl g :=
+  forall x la gamma,
+    (@isLookaheadFor g) la x gamma
+    -> exists laMap,
+      StringMap.find x tbl = Some laMap
+      /\ LookaheadMap.find la laMap = Some gamma.
+
+Definition isParseTableFor (tbl : parse_table)  (g : grammar)  := ptMinimal tbl g /\ ptComplete tbl g.
+
+Theorem parseForest_correct :
+  forall (g   : grammar)
+         (tbl : parse_table),
+    ParseTable.isParseTableFor tbl g ->
+    forall f input gamma suffix fuel,
+      parseForest tbl gamma input fuel =
+      (Some f, suffix) ->
+      exists prefix,
+        (prefix ++ suffix)%list = input /\
+        (@derivesForest g) gamma prefix f.
+Proof.
+  intros g tbl Htbl f.
+  induction f using forest_mutual_ind with
+      (P0 := fun subtrees =>
+               forall input gamma suffix fuel,
+                 parseForest tbl gamma input fuel =
+                 (Some subtrees, suffix) ->
+                 exists prefix,
+                   (prefix ++ suffix)%list = input /\
+                   (@derivesForest g) gamma prefix subtrees)
+      (P := fun tr =>
+              forall input sym suffix fuel,
+                parse tbl sym input fuel = (Some tr, suffix) ->
+                exists prefix,
+                  (prefix ++ suffix)%list = input /\
+                  (@derivesTree g) sym prefix tr).
+
+  - intros input sym suffix fuel Hparse. 
+    destruct fuel as [| fuel].
+    + inv Hparse.
+    + destruct sym as [y | x].
+      * destruct input as [| token input].
+        { inv Hparse. }
+        simpl in Hparse.
+        destruct (Utils.beqString y token) eqn:Hbeq.
+        { inv Hparse. exists [token]. split.
+          { reflexivity. }
+          apply beqString_eq in Hbeq. subst.
+          apply derivesT. }
+        inv Hparse.
+      * apply nt_derives_Node in Hparse. inv Hparse.
+
+  - intros input sym suffix fuel Hparse.
+    destruct fuel as [| fuel].
+    + inv Hparse.
+    + destruct sym as [y | x].
+      * apply t_derives_Leaf in Hparse. inv Hparse.
+      * simpl in Hparse. 
+        destruct (parseTableLookup x (peek input) tbl)
+                 as [ys |] eqn:Hlookup.
+        { destruct (parseForest tbl ys input fuel)
+                   as [subresult input'] eqn:Hforest.
+          { destruct subresult as [subtrees |].
+            { inv Hparse.
+              apply IHf in Hforest.
+              destruct Hforest as [prefix Hforest].
+              exists prefix.
+              destruct Hforest as [Happ Hderives]. split.
+              { assumption. }
+              inv Hderives.
+              { apply derivesNT with (gamma := nil).
+                { simpl in Hlookup. 
+                  apply lookup_tbl_in_grammar with
+                      (g := g)
+                      (x := s)
+                      (y := peek suffix)
+                      (gamma:=nil) in Hlookup.
+                  { assumption. }
+                  assumption. }
+                apply derivesFnil. }
+              apply derivesNT with
+                  (gamma := (hdRoot :: tlRoots)).
+              { eapply lookup_tbl_in_grammar; eassumption. }
+              { apply derivesFcons; assumption. }}
+            { inv Hparse. }}}
+        { inv Hparse. }
+
+  - intros input gamma suffix fuel HparseForest.
+    destruct fuel as [| fuel].
+    + inv HparseForest.
+    + destruct gamma as [| sym gamma'].
+      * simpl in HparseForest. inv HparseForest.
+        exists nil. split.
+        { reflexivity. }
+        apply derivesFnil.
+      * exfalso.
+        simpl in HparseForest.
+        destruct (parse tbl sym input fuel)
+          as [subresult input'].
+        destruct subresult as [lSib |].
+        { destruct (parseForest tbl gamma' input' fuel)
+            as [subresult input''].
+          destruct subresult as [rSibs |].
+          { inv HparseForest. }
+          inv HparseForest. }
+        inv HparseForest.
+
+  - intros input gamma suffix fuel HparseForest.
+    destruct fuel as [| fuel].
+    + inv HparseForest.
+    + destruct gamma as [| sym gamma'].
+      * inv HparseForest.
+      * simpl in HparseForest.
+        destruct (parse tbl sym input fuel)
+          as [subresult input'] eqn:Htree.
+        destruct subresult.
+        { destruct (parseForest tbl gamma' input' fuel)
+            as [subresult input''] eqn:Hforest.
+          destruct subresult as [rSibs |].
+          { inv HparseForest.
+            apply IHf in Htree.
+            { destruct Htree as [treePrefix Htree].
+              destruct Htree as [HappTree HderivesTree].
+              apply IHf0 in Hforest.
+              destruct Hforest as [forestPrefix Hforest].
+              destruct Hforest as [HappForest HderivesForest].
+              subst.
+              exists (treePrefix ++ forestPrefix)%list. split.
+              { rewrite app_assoc. reflexivity. }
+              apply derivesFcons.
+              { assumption. }
+              assumption. }}
+          inv HparseForest. }
+        inv HparseForest.
+Qed.
+
+
+
+Lemma lookup_exists :
+  forall x la tbl gamma,
+    parseTableLookup x la tbl = Some gamma
+    -> exists laMap,
+      StringMap.find x tbl = Some laMap
+      /\ LookaheadMap.find la laMap = Some gamma.
+Proof.
+  intros.
+  unfold parseTableLookup in H.
+  destruct (StringMap.find x tbl) as [laMap |] eqn:Hsf.
+  - exists laMap; split; trivial.
+  - inv H.
+Qed.
+
+Scheme firstprod_ind := Induction for firstProd Sort Prop
+  with firstgamma_ind := Induction for firstGamma Sort Prop
+  with firstsym_ind := Induction for firstSym Sort Prop.
+
+Lemma eof_fprod :
+  forall g la x gamma,
+    (@firstProd g) la x gamma
+    -> la = EOF
+    -> False.
+Proof.
+  intros g la x gamma H.
+  induction H using firstprod_ind with
+      (P := fun la x gamma (pf : firstProd la x gamma) =>
+              la = EOF -> False)
+      (P0 := fun la gamma (pf : firstGamma la gamma) =>
+               la = EOF -> False)
+      (P1 := fun la sym (pf : firstSym la sym) =>
+               la = EOF -> False); intros.
+  - apply IHfirstProd; trivial.
+  - apply IHfirstProd; trivial.
+  - apply IHfirstProd; trivial. 
+  - inv H.
+  - apply IHfirstProd; trivial.
+Qed.
+
+Lemma eof_fgamma :
+  forall g la gamma,
+    (@firstGamma g) la gamma
+    -> la = EOF
+    -> False.
+Proof.
+  intros g la gamma H.
+  induction H using firstgamma_ind with
+      (P := fun la x gamma (pf : firstProd la x gamma) =>
+              la = EOF -> False)
+      (P0 := fun la gamma (pf : firstGamma la gamma) =>
+               la = EOF -> False)
+      (P1 := fun la sym (pf : firstSym la sym) =>
+               la = EOF -> False); intros.
+  - apply IHfirstGamma; trivial.
+  - apply IHfirstGamma; trivial.
+  - apply IHfirstGamma; trivial. 
+  - inv H.
+  - apply IHfirstGamma; trivial.
+Qed.
+
+
+
+Lemma eof_nullable :
+  forall gamma tbl g x,
+    isParseTableFor tbl g
+    -> parseTableLookup x EOF tbl = Some gamma
+    -> exists f,
+        (@derivesForest g) gamma [] f.
+Proof.
+  induction gamma as [| sym syms]; intros.
+  - exists Fnil. constructor.
+  - apply lookup_exists in H0.
+    destruct H0 as [laMap [Hsf Hlf]].
+    destruct H as [Hmin Hcom].
+    unfold ptMinimal in Hmin.
+    apply Hmin with (la := EOF) (gamma := sym :: syms) in Hsf.
+    + destruct Hsf.
+      * apply eof_fprod in H; inv H; trivial.
+      * destruct H as [Hnp Hfp].
+        inv Hnp.
+        inv H0.
+        inv H3.
+        inv Hfp.
+Abort.
+      
+
+(* This would solve the goal *)
+Lemma gamma_gamma' :
+  forall gamma gamma' tbl g x prefix suffix fuel f f' suffix',
+    isParseTableFor tbl g
+    -> parseTableLookup x (peek (prefix ++ suffix)) tbl =
+       Some gamma'
+    -> In (x, gamma) (productions g)
+    -> parseForest tbl gamma (prefix ++ suffix) fuel =
+       (Some f, suffix)
+    -> parseForest tbl gamma' (prefix ++ suffix) fuel =
+       (Some f', suffix')
+    -> gamma = gamma'.
+Proof.
+  induction gamma as [| sym syms].
+  - induction gamma' as [| sym' syms']; intros.
+
+    + trivial.
+
+    + exfalso.
+      apply parseForest_correct with (g := g) in H2.
+      * destruct H2 as [pre [Happ Hder]].
+        assert (pre = prefix).
+        { admit. }
+        subst.
+        inv Hder.
+        simpl in *.
+        destruct H as [Hmin Hcom].
+        destruct suffix as [| tok toks].
+        -- simpl in *.
+           unfold ptMinimal in Hmin.
+           apply lookup_exists in H0.
+           destruct H0 as [laMap [Hsfind Hlfind]].
+           apply Hmin with (la := EOF)
+                           (gamma := sym' :: syms') in Hsfind.
+           ++ destruct Hsfind as [Hfi | Hfo].
+              ** apply eof_fprod in Hfi.
+                 --- inv Hfi.
+                 --- trivial.
+              ** destruct Hfo as [Hnp Hfp].
+                 inv Hfp.
+                 inv H0.
+                 --- unfold ptComplete in Hcom.
+                     assert (Hlk : (@isLookaheadFor g)  EOF (start g)
+                                                    []).
+                     { unfold isLookaheadFor.
+                       right.
+                       split.
+                       { constructor. trivial. constructor. }
+                       { constructor. trivial. constructor. }}
+                     assert (Hlk' : (@isLookaheadFor g)
+                                     EOF
+                                     (start g)
+                                     (sym' :: syms')).
+                     { unfold isLookaheadFor.
+                       right.
+                       split.
+                       { trivial. }
+                       { constructor.
+                         trivial.
+                         constructor. }}
+                     apply Hcom in Hlk.
+                     apply Hcom in Hlk'.
+                     destruct Hlk as [map [map1 map2]].
+                     destruct Hlk' as [map' [map1' map2']].
+                     congruence.
+                 --- apply eof_fgamma in H4.
+                     +++ inv H4.
+                     +++ trivial.
+                 --- assert (Hlk : (@isLookaheadFor g)
+                                     EOF
+                                     x
+                                     []).
+                     +++ unfold isLookaheadFor.
+                         right.
+                         split.
+                         *** constructor.
+                             trivial.
+                             constructor.
+                         *** constructor.
+                             trivial.
+                             eapply f_left.
+                             ---- eassumption.
+                             ---- trivial.
+                             ---- trivial.
+                     +++ assert (Hlk' : (@isLookaheadFor g)
+                                          EOF
+                                          x
+                                          (sym' :: syms')).
+                         { unfold isLookaheadFor.
+                           right.
+                           split.
+                           { trivial. }
+                           { constructor.
+                             trivial.
+                             eapply f_left; eauto. }}
+                         apply Hcom in Hlk.
+                         apply Hcom in Hlk'.
+                         destruct Hlk.
+                         destruct Hlk'.
+                         destruct H0.
+                         destruct H6.
+                         congruence.
+           ++ trivial.
+              
+        -- simpl in *.
+           unfold ptMinimal in Hmin.
+           apply lookup_exists in H0.
+           destruct H0 as [map [Hsf Hlf]].
+           apply Hmin with (la := LA tok)
+                           (gamma := sym' :: syms')
+             in Hsf.
+
+           ++ unfold ptComplete in Hcom.
+              destruct Hsf as [Hfi | Hfo].
+              ** inv Hfi.
+                 inv H0.
+                 --- inv H4.
+                     +++ assert (Hlkp : (@isLookaheadFor g)
+                                          (LA tok)
+                                          x
+                                          []).
+                         { unfold isLookaheadFor.
+                           right.
+                           split.
+                           { constructor.
+                             trivial.
+                             constructor. }
+                           { 
+                           
+                             
+
+
+                     intros.
+  destruct prefix; destruct suffix; simpl in *.
+  - (* prefix and suffix are nil *)
+    (* prove that they both derive nil? *)
+  intros tbl g x prefix suffix gamma Htbl Hlkp.
+  apply lookup_exists in Hlkp.
+  destruct Hlkp as [laMap [Hsf Hlf]].
+  pose proof Hsf as Hsf'.
+  destruct Htbl as [Hmin Hcom].
+  unfold ptMinimal in Hmin.
+  unfold ptComplete in Hcom.
+  apply Hmin with
+      (la := peek (prefix ++ suffix)) (gamma := gamma) in Hsf.
+  - destruct Hsf as [Hfirst | Hfollow].
+    + inv Hfirst; intros.
+      * destruct prefix; destruct suffix.
+        -- simpl in *.
+
+  
+  induction prefix as [| pt pts].
+  - induction suffix as [| st sts]; intros.
+    + simpl in *.
+      apply parseForest_correct with (g := g) in H1.
+      * destruct H1 as [prefix [H3 H4]].
+        assert (prefix = nil).
+        { destruct prefix; trivial; inv H3. }
+        subst.
+        clear H3.
+        apply lookup_exists in H2.
+        destruct H2 as [laMap [Hsfind Hlfind]].
+        destruct H.
+        unfold ptMinimal in H.
+        unfold ptComplete in H1.
+        apply H with (la := EOF) (gamma := gamma') in Hsfind.
+        -- destruct Hsfind.
+           ++ apply eof_fprod in H2; inv H2.
+              trivial.
+           ++ destruct H2 as [Hnp Hfp].
+              inv Hnp.
+              inv H3.
+              ** inv Hfp.
+                 inv H5.
+              
+
+
+
+
+
+             
+Lemma lookup_exists :
+  forall x la tbl gamma,
+    parseTableLookup x la tbl = Some gamma
+    -> exists laMap,
+      StringMap.find x tbl = Some laMap
+      /\ LookaheadMap.find la laMap = Some gamma.
+Proof.
+  intros.
+  unfold parseTableLookup in H.
+  destruct (StringMap.find x tbl) as [laMap |] eqn:Hsf.
+  - exists laMap; split; trivial.
+  - inv H.
+Qed.
+
+Lemma der_lookup :
+   forall tbl g,
+    isParseTableFor tbl g
+    -> forall prefix suffix x gamma fuel f gamma',
+       In (x, gamma) (productions g)
+       -> parseForest tbl gamma (app prefix suffix) fuel =
+          (Some f, suffix)
+       -> parseTableLookup x (peek (app prefix suffix)) tbl =
+          Some gamma'
+       -> gamma = gamma'.
+Proof.
+  intros tbl g Htbl prefix.
+  unfold isParseTableFor in Htbl.
+  destruct Htbl as [Hmin Hcom].
+  intros.
+  apply lkp_ex in H1.
+  destruct H1 as [laMap [Hsf Hlf]].
+  pose proof Hsf.
+  unfold ptMinimal in Hmin.
+  apply Hmin with (la := peek (app prefix suffix))
+                  (gamma := gamma') in Hsf.
+  - destruct (peek (prefix ++ suffix)) eqn:Hpeek.
+    + unfold ptComplete in Hcom.
+      apply Hcom with (la := LA s) in Hsf.
+      destruct Hsf as [laMap' [Hsf' Hlf']].
+      rewrite H1 in Hsf'.
+      inv Hsf'.
+      rewrte 
+
+  
+  induction prefix as [| pt pts]; intros.
+  - simpl in *.
+    apply lkp_ex in H1.
+    destruct H1 as [laMap [Hsf Hlf]].
+    unfold ptMinimal in Hmin.
+    unfold ptComplete in Hcom.
+    apply Hmin with (la := peek suffix) (gamma := gamma')
+      in Hsf.
+    + unfold isLookaheadFor in Hsf.
+      destruct Hsf as [Hfp | Hnp].
+      * inv Hfp.
+        inv H2.
+        -- inv H3.
+        rewrite <- H4 in Hlf.
+        
+    
+  induction gamma as [| sym syms]; intros.
+  - inv H0.
+    simpl.
+    unfold ptMinimal in Hmin.
+    unfold parseTableLookup.
+    destruct (StringMap.find x tbl) as [laMap |] eqn:Hsf.
+    + destruct (LookaheadMap.find EOF laMap)
+        as [gamma |] eqn:Hlf.
+      * destruct gamma.
+        -- trivial.
+        -- eapply Hmin with (la := EOF) (gamma := gamma)
+            in Hsf.
+           ++ unfold Hsf.
+j
+    
+    inv H0.
+    destruct Htbl with (x := x) (la := EOF) (gamma := @nil symbol)
+      as [Hmin Hcom].
+    inv H0.
+    simpl.
+    apply Hcom.
+    unfold isLookaheadFor.
+    right.
+    split.
+    + constructor.
+      * trivial.
+      * constructor.
+    + unfold parseTableLookup in Hmin.
+      destruct (StringMap.find x tbl) as [laMap |] eqn:Hsf.
+      * destruct (LookaheadMap.find EOF laMap) as [gamma |].
+        -- destruct (list_eq_dec symbol_eq_dec 
+
+    unfold parseTableLookup; unfold parseTableLookup in Hmin.
+    destruct (StringMap.find x tbl) eqn:Hsfind.
+    + destruct (LookaheadMap.find EOF t) eqn:Hlfind.
+      * 
+    
+      
+
+
+
+  unfold isParseTableFor in Htbl.
+  destruct Htbl as [Hcom Hmin].
+  destruct Hcom as [Hcomfi Hcomfo].
+  unfold ptCompleteFirst in Hcomfi.
+  unfold ptCompleteFollow in Hcomfo.
+  induction trees as [| tr trs]; intros.
+  - inv H0.
+    simpl in *.
+    inv H.
+    inv H4.
+    unfold parseTableMinimal in Hmin.
+    apply Hcomfo with (y := EOF) in H2.
+    + destruct H2 as [tMap [H2 H3]].
+      unfold parseTableLookup.
+      rewrite H2; rewrite H3.
+      trivial.
+    + constructor.
+    + apply Hmin in H2.
+      apply Hcomfo in H
+      * destruct H2.
+        -- inv H.
+           inv H0.
+           inv H1.
+        -- destruct H0.
+           unfold parseTableLookup.
+           rewrite H; rewrite H3.
+           trivial.
+      * trivial.
+    + constructor.
+    + 
+
+
+
+      
+Lemma in_grammar_lookup_tbl :
+  forall tbl g,
+    isParseTableFor tbl g
+    -> forall gamma prefix suffix x fuel f,
+      In (x, gamma) (productions g)
+      -> parseForest tbl gamma (app prefix suffix) fuel =
+         (Some f, suffix)
+      -> parseTableLookup x (peek (app prefix suffix)) tbl =
+         Some gamma.
+Proof.
+  intros tbl g Htbl gamma.
+  intros.
+  assert (H1 : exists (prefix' : list string),
+               (app prefix' suffix) = (app prefix suffix)
+               /\ (@derivesForest g) gamma prefix' f).
+  { admit. }
+  destruct H1 as [prefix' [H1 H2]].
+  assert (prefix' = prefix).
+  { admit. }
+  subst.
+  assert ((@derivesTree g) (NT x) prefix (Node x f)).
+  { eapply derivesNT; eauto. }
+  apply derives_exists in H3.
+
+(* Ultimate goal *)
+(*
+  g : grammar
+  tbl : parse_table
+  Htbl : isParseTableFor tbl g
+  s : string
+  f : forest
+  prefix, suffix : list string
+  gamma : list symbol
+  H3 : In (s, gamma) (productions g)
+  fuel : nat
+  H : parseForest tbl gamma (prefix ++ suffix) fuel =
+      (Some f, suffix)
+  gamma' : list symbol
+  Hlkp : parseTableLookup s (peek (prefix ++ suffix)) tbl =
+         Some gamma'
+  f' : forest
+  suffix' : list string
+  Hpf : parseForest tbl gamma' (prefix ++ suffix) fuel =
+        (Some f', suffix')
+  ============================
+  (Some (Node s f'), suffix') = (Some (Node s f), suffix)
+
+ *)
+
+
+
+(*
+
+case 1 -- prefix == suffix == nil
+
+In (x, gamma) (productions g)
+
+parseForest gamma nil = (Some f, nil)
+--> derivesForest gamma nil f
+
+parseTableLookup x EOF = Some gamma'
+--> we know that either EOF is in FIRST for (x, gamma')
+    (can't be true), or that gamma' is nullable and 
+    EOF is in FOLLOW for (x, gamma')
+       
+parseForest gamma' nil = (Some f', suffix')
+--> suffix' = nil
