LL1/MonotonicityLemmas.v
@@ -1,0 +1,317 @@
+Require Import List Omega String.
+Require Import Lib.Derivation Lib.Grammar Lib.Lemmas
+               Lib.ParseTree Lib.Tactics.
+Require Import LL1.CorrectnessProof. (* move lemmas out *)
+Require Import LL1.ParseTable LL1.Parser.
+
+Lemma parse_fuel_monotonic :
+  forall tr tbl sym input suffix fuel fuel2,
+    parse tbl sym input fuel = (Some tr, suffix)
+    -> fuel < fuel2
+    -> parse tbl sym input fuel2 = (Some tr, suffix).
+Proof.
+  induction tr as [ s
+                  | s f IHparseForest
+                  |
+                  | tr IHparse f IHparseForest ]
+      using tree_mutual_ind with
+      (P := fun tr =>
+              forall tbl sym input suffix fuel fuel2,
+                parse tbl sym input fuel = (Some tr, suffix)
+                -> fuel < fuel2
+                -> parse tbl sym input fuel2 =
+                   (Some tr, suffix))
+      (P0 := fun subtrees =>
+               forall tbl gamma input suffix fuel fuel2,
+                 parseForest tbl gamma input fuel =
+                 (Some subtrees, suffix)
+                 -> fuel < fuel2
+                 -> parseForest tbl gamma input fuel2 =
+                    (Some subtrees, suffix)).
+  
+  - intros tbl sym input suffix fuel fuel2 Hparse Hfuel.
+    destruct fuel.
+    + inv Hparse.
+    + destruct fuel2.
+      * inv Hfuel.
+      * destruct sym as [y | x].
+        { destruct input as [| token tokens].
+          { inv Hparse. }
+          { simpl; simpl in Hparse.
+            destruct (Utils.beqString y token).
+            { inv Hparse. reflexivity. }
+            { inv Hparse. }}}
+        { apply nt_derives_Node in Hparse. inv Hparse. }
+
+  - intros tbl sym input suffix fuel fuel2 Hparse Hfuel.
+    destruct fuel.
+    + inv Hparse.
+    + destruct fuel2.
+      * inv Hfuel.
+      * destruct sym as [y | x].
+        { apply t_derives_Leaf in Hparse. inv Hparse. }
+        { simpl; simpl in Hparse.
+          destruct (parseTableLookup x (peek input) tbl)
+            as [gamma |] eqn:Hlookup.
+          { destruct (parseForest tbl gamma input fuel)
+              as (subresult, input') eqn:Hpf.
+            destruct subresult as [subtrees |].
+            { inv Hparse.
+              apply IHparseForest with (fuel2 := fuel2)in Hpf;
+              clear IHparseForest.
+              { destruct (parseForest tbl gamma input fuel2)
+                  as (subresult, input') eqn:Hpf2.
+                destruct subresult as [subtrees |].
+                { congruence. }
+                { inv Hpf. }}
+              { apply lt_S_n. assumption. }}
+            { inv Hparse. }}
+          { inv Hparse. }}
+
+  - intros tbl gamma input suffix fuel fuel2 Hparse Hfuel.
+    destruct fuel.
+    + inv Hparse.
+    + destruct fuel2.
+      * inv Hfuel.
+      * destruct gamma as [| sym syms].
+        { simpl. inv Hparse. reflexivity. }
+        (* Maybe prove in a separate lemma that 
+           a non-empty gamma never derives Fnil *)
+        { simpl in Hparse.
+          destruct (parse tbl sym input fuel)
+            as (subresult, input').
+          destruct subresult as [lSib |].
+          { destruct (parseForest tbl syms input' fuel)
+              as (subresult, input'').
+            destruct subresult as [rSibs |].
+            { inv Hparse. }
+            { inv Hparse. }}
+          { inv Hparse. }}
+
+  - intros tbl gamma input suffix fuel fuel2 Hparse Hfuel.
+    destruct fuel.
+    + inv Hparse.
+    + destruct fuel2.
+      * inv Hfuel.
+      * destruct gamma as [| sym syms].
+        { inv Hparse. }
+        { simpl; simpl in Hparse.
+          destruct (parse tbl sym input fuel)
+            as (subresult, input') eqn:HparseFuel.
+          { destruct subresult as [lSib |].
+            { destruct (parseForest tbl syms input' fuel)
+                as (subresult, input'') eqn:HparseForestFuel.
+              destruct subresult as [rSibs |].
+              { destruct (parse tbl sym input fuel2)
+                  as (subresult, input2') eqn:HparseFuel2.
+                { destruct subresult as [lSib2 |].
+                  { destruct (parseForest tbl syms input2' fuel2) as (subresult, input2'') eqn:HparseForestFuel2.
+                    destruct subresult as [rSibs2 |].
+                    { inv Hparse.
+                      apply IHparse with (fuel2 := fuel2)
+                        in HparseFuel.
+                      { rewrite HparseFuel in HparseFuel2.
+                        inv HparseFuel2.
+                        apply IHparseForest
+                          with (fuel2 := fuel2)
+                          in HparseForestFuel.
+                        { rewrite HparseForestFuel in HparseForestFuel2.
+                          inv HparseForestFuel2.
+                          reflexivity. }
+                        { omega. }}
+                      { omega. }}
+                    { inv Hparse.
+                      apply IHparse
+                        with (fuel2 := fuel2)
+                        in HparseFuel.
+                      { rewrite HparseFuel in HparseFuel2.
+                        inv HparseFuel2.
+                        apply IHparseForest
+                          with (fuel2 := fuel2)
+                        in HparseForestFuel.
+                        { rewrite HparseForestFuel
+                          in HparseForestFuel2.
+                          inv HparseForestFuel2. }
+                        { omega. }}
+                      { omega. }}}
+                  { inv Hparse.
+                    apply IHparse
+                      with (fuel2 := fuel2)
+                      in HparseFuel.
+                    { rewrite HparseFuel in HparseFuel2.
+                      inv HparseFuel2. }
+                    { omega. }}}}
+              { inv Hparse. }}
+            { inv Hparse. }}}
+Qed.
+
+Lemma parseForest_fuel_monotonic :
+  forall sts tbl gamma input suffix fuel fuel2,
+    parseForest tbl gamma input fuel = (Some sts, suffix)
+    -> fuel < fuel2
+    -> parseForest tbl gamma input fuel2 = (Some sts, suffix).
+Proof.
+  induction sts as [ s
+                   | s f IHparseForest
+                   |
+                   | tr IHparse f IHparseForest ]
+      using forest_mutual_ind with
+      (P := fun tr =>
+              forall tbl sym input suffix fuel fuel2,
+                parse tbl sym input fuel = (Some tr, suffix)
+                -> fuel < fuel2
+                -> parse tbl sym input fuel2 =
+                   (Some tr, suffix))
+      (P0 := fun subtrees =>
+               forall tbl gamma input suffix fuel fuel2,
+                 parseForest tbl gamma input fuel =
+                 (Some subtrees, suffix)
+                 -> fuel < fuel2
+                 -> parseForest tbl gamma input fuel2 =
+                    (Some subtrees, suffix)).
+  
+  - intros tbl sym input suffix fuel fuel2 Hparse Hfuel.
+    destruct fuel.
+    + inv Hparse.
+    + destruct fuel2.
+      * inv Hfuel.
+      * destruct sym as [y | x].
+        { destruct input as [| token tokens].
+          { inv Hparse. }
+          { simpl; simpl in Hparse.
+            destruct (Utils.beqString y token).
+            { inv Hparse. reflexivity. }
+            { inv Hparse. }}}
+        { apply nt_derives_Node in Hparse. inv Hparse. }
+
+  - intros tbl sym input suffix fuel fuel2 Hparse Hfuel.
+    destruct fuel.
+    + inv Hparse.
+    + destruct fuel2.
+      * inv Hfuel.
+      * destruct sym as [y | x].
+        { apply t_derives_Leaf in Hparse. inv Hparse. }
+        { simpl; simpl in Hparse.
+          destruct (parseTableLookup x (peek input) tbl)
+            as [gamma |] eqn:Hlookup.
+          { destruct (parseForest tbl gamma input fuel)
+              as (subresult, input') eqn:Hpf.
+            destruct subresult as [subtrees |].
+            { inv Hparse.
+              apply IHparseForest with (fuel2 := fuel2)in Hpf;
+              clear IHparseForest.
+              { destruct (parseForest tbl gamma input fuel2)
+                  as (subresult, input') eqn:Hpf2.
+                destruct subresult as [subtrees |].
+                { congruence. }
+                { inv Hpf. }}
+              { apply lt_S_n. assumption. }}
+            { inv Hparse. }}
+          { inv Hparse. }}
+
+  - intros tbl gamma input suffix fuel fuel2 Hparse Hfuel.
+    destruct fuel.
+    + inv Hparse.
+    + destruct fuel2.
+      * inv Hfuel.
+      * destruct gamma as [| sym syms].
+        { simpl. inv Hparse. reflexivity. }
+        (* Maybe prove in a separate lemma that 
+           a non-empty gamma never derives Fnil *)
+        { simpl in Hparse.
+          destruct (parse tbl sym input fuel)
+            as (subresult, input').
+          destruct subresult as [lSib |].
+          { destruct (parseForest tbl syms input' fuel)
+              as (subresult, input'').
+            destruct subresult as [rSibs |].
+            { inv Hparse. }
+            { inv Hparse. }}
+          { inv Hparse. }}
+
+  - intros tbl gamma input suffix fuel fuel2 Hparse Hfuel.
+    destruct fuel.
+    + inv Hparse.
+    + destruct fuel2.
+      * inv Hfuel.
+      * destruct gamma as [| sym syms].
+        { inv Hparse. }
+        { simpl; simpl in Hparse.
+          destruct (parse tbl sym input fuel)
+            as (subresult, input') eqn:HparseFuel.
+          { destruct subresult as [lSib |].
+            { destruct (parseForest tbl syms input' fuel)
+                as (subresult, input'') eqn:HparseForestFuel.
+              destruct subresult as [rSibs |].
+              { destruct (parse tbl sym input fuel2)
+                  as (subresult, input2') eqn:HparseFuel2.
+                { destruct subresult as [lSib2 |].
+                  { destruct (parseForest tbl syms input2' fuel2) as (subresult, input2'') eqn:HparseForestFuel2.
+                    destruct subresult as [rSibs2 |].
+                    { inv Hparse.
+                      apply IHparse with (fuel2 := fuel2)
+                        in HparseFuel.
+                      { rewrite HparseFuel in HparseFuel2.
+                        inv HparseFuel2.
+                        apply IHparseForest
+                          with (fuel2 := fuel2)
+                          in HparseForestFuel.
+                        { rewrite HparseForestFuel in HparseForestFuel2.
+                          inv HparseForestFuel2.
+                          reflexivity. }
+                        { omega. }}
+                      { omega. }}
+                    { inv Hparse.
+                      apply IHparse
+                        with (fuel2 := fuel2)
+                        in HparseFuel.
+                      { rewrite HparseFuel in HparseFuel2.
+                        inv HparseFuel2.
+                        apply IHparseForest
+                          with (fuel2 := fuel2)
+                        in HparseForestFuel.
+                        { rewrite HparseForestFuel
+                          in HparseForestFuel2.
+                          inv HparseForestFuel2. }
+                        { omega. }}
+                      { omega. }}}
+                  { inv Hparse.
+                    apply IHparse
+                      with (fuel2 := fuel2)
+                      in HparseFuel.
+                    { rewrite HparseFuel in HparseFuel2.
+                      inv HparseFuel2. }
+                    { omega. }}}}
+              { inv Hparse. }}
+            { inv Hparse. }}}
+Qed. (* Hmm...same proof as the one for parse! *)
+
+Lemma parse_fuel_max :
+  forall fuel tbl sym input fuel2 tr suffix,
+    parse tbl sym input fuel = (Some tr, suffix) ->
+    parse tbl sym input (max fuel fuel2) = (Some tr, suffix).
+Proof.
+  intros. 
+  pose proof (Max.max_spec fuel fuel2) as H_max_spec.
+  destruct H_max_spec.
+  - destruct H0. rewrite H1.
+    eapply parse_fuel_monotonic.
+    + eassumption.
+    + assumption.
+  - destruct H0. rewrite H1. assumption.
+Qed.
+
+Lemma parseForest_fuel_max :
+  forall tbl gamma input fuel fuel2 sts suffix,
+    parseForest tbl gamma input fuel = (Some sts, suffix)
+    -> parseForest tbl gamma input (max fuel fuel2) =
+       (Some sts, suffix).
+Proof.
+  intros. pose proof (Max.max_spec fuel fuel2) as H_max_spec.
+  destruct H_max_spec.
+  - destruct H0. rewrite H1.
+    eapply parseForest_fuel_monotonic.
+    + eassumption.
+    + assumption.
+  - destruct H0. rewrite H1. assumption.
+Qed.
